CPolyEquiv/CPolyEquiv.lean
@@ -1,4 +1,0 @@
-import CPolyEquiv.Generated
-import CPolyEquiv.Equiv
-import CPolyEquiv.EquivMl
-import CPolyEquiv.Check
